LambdaS5/coq/LjsRulesCorrectExpressions.v
@@ -76,6 +76,8 @@ Proof.
     repeat ljs_autoforward.
     inverts Hvrel2.
     jauto_js.
+
+
     skip.
     skip.
     skip.
